guard pages WIP: src/SlabsFree WIP

src/SlabsFree.fst
@@ -450,8 +450,6 @@ let deallocate_slab_aux_1
   )
 #pop-options
 
-// checkpoint
-
 inline_for_extraction noextract
 let deallocate_slab_aux_2_empty
   (size_class: sc)
@@ -459,12 +457,10 @@ let deallocate_slab_aux_2_empty
   (md_bm_region: array U64.t{A.length md_bm_region = U32.v metadata_max * 4})
   (md_region: array AL.cell{A.length md_region = U32.v metadata_max})
   (md_count: ref U32.t)
-  (r1 r2 r3: ref US.t)
+  (r1 r2 r3 r4:  ref US.t)
   (md_count_v: U32.t{U32.v md_count_v <= U32.v metadata_max})
   (md_region_lv: G.erased (Seq.lseq AL.status (U32.v md_count_v)))
-  (idx1: US.t)
-  (idx2: US.t)
-  (idx3: US.t)
+  (idx1 idx2 idx3 idx4: US.t)
   (pos: US.t{pos <> AL.null_ptr /\ US.v pos < U32.v md_count_v})
   : Steel unit
   (
@@ -472,9 +468,10 @@ let deallocate_slab_aux_2_empty
     vptr r1 `star`
     vptr r2 `star`
     vptr r3 `star`
-    (AL.varraylist pred1 pred2 pred3
+    vptr r4 `star`
+    (AL.varraylist pred1 pred2 pred3 pred4
       (A.split_l md_region (u32_to_sz md_count_v))
-      (US.v idx1) (US.v idx2) (US.v idx3)) `star`
+      (US.v idx1) (US.v idx2) (US.v idx3) (US.v idx4)) `star`
     starseq
       #(pos:U32.t{U32.v pos < U32.v md_count_v})
       #(t size_class)
@@ -486,17 +483,20 @@ let deallocate_slab_aux_2_empty
     vrefinedep
       (vptr md_count)
       vrefinedep_prop
-      (left_vprop size_class slab_region md_bm_region md_region r1 r2 r3)
+      (left_vprop size_class slab_region md_bm_region md_region r1 r2 r3 r4)
   )
   (requires fun h0 ->
-    let gs0 = AL.v_arraylist pred1 pred2 pred3 (A.split_l md_region (u32_to_sz md_count_v)) (US.v idx1) (US.v idx2) (US.v idx3) h0 in
+    let gs0 = AL.v_arraylist pred1 pred2 pred3 pred4
+      (A.split_l md_region (u32_to_sz md_count_v))
+      (US.v idx1) (US.v idx2) (US.v idx3) (US.v idx4) h0 in
     U32.v md_count_v <> AL.null /\
     sel md_count h0 == md_count_v /\
     sel r1 h0 == idx1 /\
     sel r2 h0 == idx2 /\
     sel r3 h0 == idx3 /\
+    sel r4 h0 == idx4 /\
     ALG.dataify gs0 `Seq.equal` G.reveal md_region_lv /\
-    ALG.partition #AL.status gs0 (US.v idx1) (US.v idx2) (US.v idx3) /\
+    ALG.partition #AL.status gs0 (US.v idx1) (US.v idx2) (US.v idx3) (US.v idx4) /\
     Seq.index (G.reveal md_region_lv) (US.v pos) = 1ul
   )
   (ensures fun _ _ h1 ->
@@ -504,32 +504,36 @@ let deallocate_slab_aux_2_empty
       = h1 (vrefinedep
       (vptr md_count)
       vrefinedep_prop
-      (left_vprop size_class slab_region md_bm_region md_region r1 r2 r3)
+      (left_vprop size_class slab_region md_bm_region md_region r1 r2 r3 r4)
     ) in
     md_count_v == dfst blob1)
   =
-  (**) let gs0 = gget (AL.varraylist pred1 pred2 pred3 (A.split_l md_region (u32_to_sz md_count_v)) (US.v idx1) (US.v idx2) (US.v idx3)) in
+  (**) let gs0 = gget (AL.varraylist pred1 pred2 pred3 pred4
+    (A.split_l md_region (u32_to_sz md_count_v))
+    (US.v idx1) (US.v idx2) (US.v idx3) (US.v idx4)) in
   //assert (ALG.partition #AL.status gs0 (US.v idx1) (US.v idx2) (US.v idx3));
   (**) ALG.lemma_dataify_index #AL.status gs0 (US.v pos);
-  (**) lemma_partition_and_pred_implies_mem2 (US.v idx1) (US.v idx2) (US.v idx3) gs0 (US.v pos);
+  (**) lemma_partition_and_pred_implies_mem2 (US.v idx1) (US.v idx2) (US.v idx3) (US.v idx4) gs0 (US.v pos);
   assert (ALG.mem #AL.status (US.v pos) (US.v idx2) gs0);
 
-  let idx2' = AL.remove2 #pred1 #pred2 #pred3
+  let idx2' = AL.remove2 #pred1 #pred2 #pred3 #pred4
     (A.split_l md_region (u32_to_sz md_count_v))
-    (G.hide (US.v idx1)) idx2 (G.hide (US.v idx3)) pos in
-  AL.insert1 #pred1 #pred2 #pred3
+    (G.hide (US.v idx1)) idx2 (G.hide (US.v idx3)) (G.hide (US.v idx4)) pos in
+  AL.insert1 #pred1 #pred2 #pred3 #pred4
     (A.split_l md_region (u32_to_sz md_count_v))
-    idx1 (G.hide (US.v idx2')) (G.hide (US.v idx3)) pos 0ul;
+    idx1 (G.hide (US.v idx2')) (G.hide (US.v idx3)) (G.hide (US.v idx4)) pos 0ul;
   write r2 idx2';
   write r1 pos;
 
-  (**) let gs1 = gget (AL.varraylist pred1 pred2 pred3 (A.split_l md_region (u32_to_sz md_count_v)) (US.v pos) (US.v idx2') (US.v idx3)) in
-  assert (ALG.ptrs_all #AL.status (US.v idx1) (US.v idx2) (US.v idx3) gs0 `FStar.FiniteSet.Base.equal`
-          ALG.ptrs_all #AL.status (US.v pos) (US.v idx2') (US.v idx3) gs1);
+  (**) let gs1 = gget (AL.varraylist pred1 pred2 pred3 pred4
+    (A.split_l md_region (u32_to_sz md_count_v))
+    (US.v pos) (US.v idx2') (US.v idx3) (US.v idx4)) in
+  assert (ALG.ptrs_all #AL.status (US.v idx1) (US.v idx2) (US.v idx3) (US.v idx4) gs0 `FStar.FiniteSet.Base.equal`
+          ALG.ptrs_all #AL.status (US.v pos) (US.v idx2') (US.v idx3) (US.v idx4) gs1);
 
-  (**) pack_3 size_class slab_region md_bm_region md_region md_count r1 r2 r3
+  (**) pack_3 size_class slab_region md_bm_region md_region md_count r1 r2 r3 r4
     md_count_v (G.hide (Seq.upd (G.reveal md_region_lv) (US.v pos) 0ul))
-    pos idx2' idx3
+    pos idx2' idx3 idx4
 
 inline_for_extraction noextract
 let deallocate_slab_aux_2_partial
@@ -538,12 +542,10 @@ let deallocate_slab_aux_2_partial
   (md_bm_region: array U64.t{A.length md_bm_region = U32.v metadata_max * 4})
   (md_region: array AL.cell{A.length md_region = U32.v metadata_max})
   (md_count: ref U32.t)
-  (r1 r2 r3: ref US.t)
+  (r1 r2 r3 r4: ref US.t)
   (md_count_v: U32.t{U32.v md_count_v <= U32.v metadata_max})
   (md_region_lv: G.erased (Seq.lseq AL.status (U32.v md_count_v)))
-  (idx1: US.t)
-  (idx2: US.t)
-  (idx3: US.t)
+  (idx1 idx2 idx3 idx4: US.t)
   (pos: US.t{US.v pos < U32.v md_count_v})
   : Steel unit
   (
@@ -551,9 +553,10 @@ let deallocate_slab_aux_2_partial
     vptr r1 `star`
     vptr r2 `star`
     vptr r3 `star`
-    (AL.varraylist pred1 pred2 pred3
+    vptr r4 `star`
+    (AL.varraylist pred1 pred2 pred3 pred4
       (A.split_l md_region (u32_to_sz md_count_v))
-      (US.v idx1) (US.v idx2) (US.v idx3)) `star`
+      (US.v idx1) (US.v idx2) (US.v idx3) (US.v idx4)) `star`
     starseq
       #(pos:U32.t{U32.v pos < U32.v md_count_v})
       #(t size_class)
@@ -565,17 +568,20 @@ let deallocate_slab_aux_2_partial
     vrefinedep
       (vptr md_count)
       vrefinedep_prop
-      (left_vprop size_class slab_region md_bm_region md_region r1 r2 r3)
+      (left_vprop size_class slab_region md_bm_region md_region r1 r2 r3 r4)
   )
   (requires fun h0 ->
-    let gs0 = AL.v_arraylist pred1 pred2 pred3 (A.split_l md_region (u32_to_sz md_count_v)) (US.v idx1) (US.v idx2) (US.v idx3) h0 in
+    let gs0 = AL.v_arraylist pred1 pred2 pred3 pred4
+      (A.split_l md_region (u32_to_sz md_count_v))
+      (US.v idx1) (US.v idx2) (US.v idx3) (US.v idx4) h0 in
     U32.v md_count_v <> AL.null /\
     sel md_count h0 == md_count_v /\
     sel r1 h0 == idx1 /\
     sel r2 h0 == idx2 /\
     sel r3 h0 == idx3 /\
+    sel r4 h0 == idx4 /\
     ALG.dataify gs0 `Seq.equal` G.reveal md_region_lv /\
-    ALG.partition #AL.status gs0 (US.v idx1) (US.v idx2) (US.v idx3) /\
+    ALG.partition #AL.status gs0 (US.v idx1) (US.v idx2) (US.v idx3) (US.v idx4) /\
     Seq.index (G.reveal md_region_lv) (US.v pos) = 1ul
   )
   (ensures fun _ _ h1 ->
@@ -583,13 +589,13 @@ let deallocate_slab_aux_2_partial
       = h1 (vrefinedep
       (vptr md_count)
       vrefinedep_prop
-      (left_vprop size_class slab_region md_bm_region md_region r1 r2 r3)
+      (left_vprop size_class slab_region md_bm_region md_region r1 r2 r3 r4)
     ) in
     md_count_v == dfst blob1)
   =
-  (**) pack_3 size_class slab_region md_bm_region md_region md_count r1 r2 r3
+  (**) pack_3 size_class slab_region md_bm_region md_region md_count r1 r2 r3 r4
     md_count_v md_region_lv
-    idx1 idx2 idx3
+    idx1 idx2 idx3 idx4
 
 inline_for_extraction noextract
 let deallocate_slab_aux_2_fail
@@ -599,12 +605,10 @@ let deallocate_slab_aux_2_fail
   (md_bm_region: array U64.t{A.length md_bm_region = U32.v metadata_max * 4})
   (md_region: array AL.cell{A.length md_region = U32.v metadata_max})
   (md_count: ref U32.t)
-  (r1 r2 r3: ref US.t)
+  (r1 r2 r3 r4: ref US.t)
   (md_count_v: U32.t{U32.v md_count_v <= U32.v metadata_max})
   (md_region_lv: G.erased (Seq.lseq AL.status (U32.v md_count_v)))
-  (idx1: US.t)
-  (idx2: US.t)
-  (idx3: US.t)
+  (idx1 idx2 idx3 idx4: US.t)
   (pos: US.t{pos <> AL.null_ptr /\ US.v pos < U32.v md_count_v})
   : SteelGhost unit opened
   (
@@ -615,9 +619,10 @@ let deallocate_slab_aux_2_fail
     vptr r1 `star`
     vptr r2 `star`
     vptr r3 `star`
-    (AL.varraylist pred1 pred2 pred3
+    vptr r4 `star`
+    (AL.varraylist pred1 pred2 pred3 pred4
       (A.split_l md_region (u32_to_sz md_count_v))
-      (US.v idx1) (US.v idx2) (US.v idx3)) `star`
+      (US.v idx1) (US.v idx2) (US.v idx3) (US.v idx4)) `star`
     starseq
       #(pos:U32.t{U32.v pos < U32.v md_count_v})
       #(t size_class)
@@ -635,10 +640,12 @@ let deallocate_slab_aux_2_fail
     vrefinedep
       (vptr md_count)
       vrefinedep_prop
-      (left_vprop size_class slab_region md_bm_region md_region r1 r2 r3)
+      (left_vprop size_class slab_region md_bm_region md_region r1 r2 r3 r4)
   )
   (requires fun h0 ->
-    let gs0 = AL.v_arraylist pred1 pred2 pred3 (A.split_l md_region (u32_to_sz md_count_v)) (US.v idx1) (US.v idx2) (US.v idx3) h0 in
+    let gs0 = AL.v_arraylist pred1 pred2 pred3 pred4
+      (A.split_l md_region (u32_to_sz md_count_v))
+      (US.v idx1) (US.v idx2) (US.v idx3) (US.v idx4) h0 in
     let md_blob : t_of (slab_vprop size_class
       (slab_array slab_region (US.sizet_to_uint32 pos))
       (md_bm_array md_bm_region (US.sizet_to_uint32 pos)))
@@ -652,8 +659,9 @@ let deallocate_slab_aux_2_fail
     sel r1 h0 == idx1 /\
     sel r2 h0 == idx2 /\
     sel r3 h0 == idx3 /\
+    sel r4 h0 == idx4 /\
     ALG.dataify gs0 `Seq.equal` Ghost.reveal md_region_lv /\
-    ALG.partition #AL.status gs0 (US.v idx1) (US.v idx2) (US.v idx3) /\
+    ALG.partition #AL.status gs0 (US.v idx1) (US.v idx2) (US.v idx3) (US.v idx4) /\
     Seq.index (G.reveal md_region_lv) (US.v pos) = 1ul
   )
   (ensures fun _ _ h1 ->
@@ -661,7 +669,7 @@ let deallocate_slab_aux_2_fail
       = h1 (vrefinedep
       (vptr md_count)
       vrefinedep_prop
-      (left_vprop size_class slab_region md_bm_region md_region r1 r2 r3)
+      (left_vprop size_class slab_region md_bm_region md_region r1 r2 r3 r4)
     ) in
     md_count_v == dfst blob1)
   =
@@ -680,12 +688,9 @@ let deallocate_slab_aux_2_fail
     (f_lemma size_class slab_region md_bm_region md_count_v md_region_lv)
     (SeqUtils.init_u32_refined (U32.v md_count_v))
     (US.v pos);
-  pack_3 size_class slab_region md_bm_region md_region md_count r1 r2 r3
+  pack_3 size_class slab_region md_bm_region md_region md_count r1 r2 r3 r4
     md_count_v md_region_lv
-    idx1 idx2 idx3
-
-
-
+    idx1 idx2 idx3 idx4
 
 #restart-solver
 
@@ -698,10 +703,10 @@ let deallocate_slab_aux_2
   (md_bm_region: array U64.t{A.length md_bm_region = U32.v metadata_max * 4})
   (md_region: array AL.cell{A.length md_region = U32.v metadata_max})
   (md_count: ref U32.t)
-  (r1 r2 r3: ref US.t)
+  (r1 r2 r3 r4: ref US.t)
   (md_count_v: U32.t{U32.v md_count_v <= U32.v metadata_max})
   (md_region_lv: G.erased (Seq.lseq AL.status (U32.v md_count_v)))
-  (idx1 idx2 idx3: US.t)
+  (idx1 idx2 idx3 idx4: US.t)
   (pos: US.t{US.v pos < U32.v md_count_v})
   : Steel bool
   (
@@ -710,9 +715,10 @@ let deallocate_slab_aux_2
     vptr r1 `star`
     vptr r2 `star`
     vptr r3 `star`
-    (AL.varraylist pred1 pred2 pred3
+    vptr r4 `star`
+    (AL.varraylist pred1 pred2 pred3 pred4
       (A.split_l md_region (u32_to_sz md_count_v))
-      (US.v idx1) (US.v idx2) (US.v idx3)) `star`
+      (US.v idx1) (US.v idx2) (US.v idx3) (US.v idx4)) `star`
     starseq
       #(pos:U32.t{U32.v pos < U32.v md_count_v})
       #(t size_class)
@@ -725,10 +731,12 @@ let deallocate_slab_aux_2
     vrefinedep
       (vptr md_count)
       vrefinedep_prop
-      (left_vprop size_class slab_region md_bm_region md_region r1 r2 r3)
+      (left_vprop size_class slab_region md_bm_region md_region r1 r2 r3 r4)
   )
   (requires fun h0 ->
-    let gs0 = AL.v_arraylist pred1 pred2 pred3 (A.split_l md_region (u32_to_sz md_count_v)) (US.v idx1) (US.v idx2) (US.v idx3) h0 in
+    let gs0 = AL.v_arraylist pred1 pred2 pred3 pred4
+      (A.split_l md_region (u32_to_sz md_count_v))
+      (US.v idx1) (US.v idx2) (US.v idx3) (US.v idx4) h0 in
     let arr' = slab_array slab_region (US.sizet_to_uint32 pos) in
     let diff = A.offset (A.ptr_of ptr) - A.offset (A.ptr_of arr') in
     same_base_array arr' ptr /\
@@ -740,8 +748,9 @@ let deallocate_slab_aux_2
     sel r1 h0 == idx1 /\
     sel r2 h0 == idx2 /\
     sel r3 h0 == idx3 /\
+    sel r4 h0 == idx4 /\
     ALG.dataify gs0 `Seq.equal` G.reveal md_region_lv /\
-    ALG.partition #AL.status gs0 (US.v idx1) (US.v idx2) (US.v idx3) /\
+    ALG.partition #AL.status gs0 (US.v idx1) (US.v idx2) (US.v idx3) (US.v idx4) /\
     Seq.index (G.reveal md_region_lv) (US.v pos) = 1ul
   )
   (ensures fun _ _ h1 ->
@@ -749,7 +758,7 @@ let deallocate_slab_aux_2
       = h1 (vrefinedep
       (vptr md_count)
       vrefinedep_prop
-      (left_vprop size_class slab_region md_bm_region md_region r1 r2 r3)
+      (left_vprop size_class slab_region md_bm_region md_region r1 r2 r3 r4)
     ) in
     md_count_v == dfst blob1)
   =
@@ -779,15 +788,15 @@ let deallocate_slab_aux_2
       (slab_array slab_region (US.sizet_to_uint32 pos)) in
     if cond then (
       (**) pack_slab_starseq size_class
-        slab_region md_bm_region md_region md_count r1 r2 r3
+        slab_region md_bm_region md_region md_count r1 r2 r3 r4
         md_count_v md_region_lv pos 0ul;
       deallocate_slab_aux_2_empty size_class
-        slab_region md_bm_region md_region md_count r1 r2 r3
-        md_count_v md_region_lv idx1 idx2 idx3 pos;
+        slab_region md_bm_region md_region md_count r1 r2 r3 r4
+        md_count_v md_region_lv idx1 idx2 idx3 idx4 pos;
       return b
     ) else (
       (**) pack_slab_starseq size_class
-        slab_region md_bm_region md_region md_count r1 r2 r3
+        slab_region md_bm_region md_region md_count r1 r2 r3 r4
         md_count_v md_region_lv pos 1ul;
       assert (Seq.upd (G.reveal md_region_lv) (US.v pos) 1ul `Seq.equal` md_region_lv);
     (**) starseq_weakening
@@ -801,19 +810,20 @@ let deallocate_slab_aux_2
       (SeqUtils.init_u32_refined (U32.v md_count_v))
       (SeqUtils.init_u32_refined (U32.v md_count_v));
       deallocate_slab_aux_2_partial size_class
-        slab_region md_bm_region md_region md_count r1 r2 r3
-        md_count_v md_region_lv idx1 idx2 idx3 pos;
+        slab_region md_bm_region md_region md_count r1 r2 r3 r4
+        md_count_v md_region_lv idx1 idx2 idx3 idx4 pos;
       return b
     )
   ) else (
     deallocate_slab_aux_2_fail size_class
-      slab_region md_bm_region md_region md_count r1 r2 r3
-      md_count_v md_region_lv idx1 idx2 idx3 pos;
+      slab_region md_bm_region md_region md_count r1 r2 r3 r4
+      md_count_v md_region_lv idx1 idx2 idx3 idx4 pos;
     return b
   )
 #pop-options
 
 #restart-solver
+
 inline_for_extraction noextract
 let deallocate_slab_fail
   (ptr: array U8.t)
@@ -822,10 +832,10 @@ let deallocate_slab_fail
   (md_bm_region: array U64.t{A.length md_bm_region = U32.v metadata_max * 4})
   (md_region: array AL.cell{A.length md_region = U32.v metadata_max})
   (md_count: ref U32.t)
-  (r1 r2 r3: ref US.t)
+  (r1 r2 r3 r4: ref US.t)
   (md_count_v: U32.t{U32.v md_count_v <= U32.v metadata_max})
   (md_region_lv: G.erased (Seq.lseq AL.status (U32.v md_count_v)))
-  (idx1 idx2 idx3: US.t)
+  (idx1 idx2 idx3 idx4: US.t)
   : Steel bool
   (
     A.varray ptr `star`
@@ -833,10 +843,11 @@ let deallocate_slab_fail
     vptr r1 `star`
     vptr r2 `star`
     vptr r3 `star`
+    vptr r4 `star`
     right_vprop (A.split_r slab_region 0sz) md_bm_region md_region md_count_v `star`
-    (AL.varraylist pred1 pred2 pred3
+    (AL.varraylist pred1 pred2 pred3 pred4
       (A.split_l md_region (u32_to_sz md_count_v))
-      (US.v idx1) (US.v idx2) (US.v idx3)) `star`
+      (US.v idx1) (US.v idx2) (US.v idx3) (US.v idx4)) `star`
     starseq
       #(pos:U32.t{U32.v pos < U32.v md_count_v})
       #(t size_class)
@@ -850,30 +861,33 @@ let deallocate_slab_fail
     vrefinedep
       (vptr md_count)
       vrefinedep_prop
-      (size_class_vprop_aux size_class slab_region md_bm_region md_region r1 r2 r3)
+      (size_class_vprop_aux size_class slab_region md_bm_region md_region r1 r2 r3 r4)
   )
   (requires fun h0 ->
-    let gs0 = AL.v_arraylist pred1 pred2 pred3 (A.split_l md_region (u32_to_sz md_count_v)) (US.v idx1) (US.v idx2) (US.v idx3) h0 in
+    let gs0 = AL.v_arraylist pred1 pred2 pred3 pred4
+      (A.split_l md_region (u32_to_sz md_count_v))
+      (US.v idx1) (US.v idx2) (US.v idx3) (US.v idx4) h0 in
     (U32.v page_size) % (U32.v size_class) = 0 /\
     sel r1 h0 == idx1 /\
     sel r2 h0 == idx2 /\
     sel r3 h0 == idx3 /\
+    sel r4 h0 == idx4 /\
     U32.v md_count_v <> AL.null /\
     md_count_v == sel md_count h0 /\
     ALG.dataify gs0 `Seq.equal` G.reveal md_region_lv /\
-    ALG.partition #AL.status gs0 (US.v idx1) (US.v idx2) (US.v idx3)
+    ALG.partition #AL.status gs0 (US.v idx1) (US.v idx2) (US.v idx3) (US.v idx4)
    )
   (ensures fun _ _ _ -> True)
   =
   let b = false in
   pack_3 size_class
     (A.split_r slab_region 0sz) md_bm_region md_region
-    md_count r1 r2 r3
+    md_count r1 r2 r3 r4
     md_count_v md_region_lv
-    idx1 idx2 idx3;
+    idx1 idx2 idx3 idx4;
   pack_right_and_refactor_vrefine_dep
     size_class slab_region md_bm_region md_region md_count
-    r1 r2 r3 md_count_v;
+    r1 r2 r3 r4 md_count_v;
   change_equal_slprop
     (A.varray ptr)
     (if b then emp else A.varray ptr);
@@ -888,10 +902,10 @@ let deallocate_slab'
   (md_bm_region: array U64.t{A.length md_bm_region = U32.v metadata_max * 4})
   (md_region: array AL.cell{A.length md_region = U32.v metadata_max})
   (md_count: ref U32.t)
-  (r1 r2 r3: ref US.t)
+  (r1 r2 r3 r4: ref US.t)
   (md_count_v: U32.t{U32.v md_count_v <= U32.v metadata_max})
   (md_region_lv: G.erased (Seq.lseq AL.status (U32.v md_count_v)))
-  (idx1 idx2 idx3: US.t)
+  (idx1 idx2 idx3 idx4: US.t)
   (diff: UP.t)
   : Steel bool
   (
@@ -900,10 +914,11 @@ let deallocate_slab'
     vptr r1 `star`
     vptr r2 `star`
     vptr r3 `star`
+    vptr r4 `star`
     right_vprop (A.split_r slab_region 0sz) md_bm_region md_region md_count_v `star`
-    (AL.varraylist pred1 pred2 pred3
+    (AL.varraylist pred1 pred2 pred3 pred4
       (A.split_l md_region (u32_to_sz md_count_v))
-      (US.v idx1) (US.v idx2) (US.v idx3)) `star`
+      (US.v idx1) (US.v idx2) (US.v idx3) (US.v idx4)) `star`
     starseq
       #(pos:U32.t{U32.v pos < U32.v md_count_v})
       #(t size_class)
@@ -917,10 +932,12 @@ let deallocate_slab'
     vrefinedep
       (vptr md_count)
       vrefinedep_prop
-      (size_class_vprop_aux size_class slab_region md_bm_region md_region r1 r2 r3)
+      (size_class_vprop_aux size_class slab_region md_bm_region md_region r1 r2 r3 r4)
   )
   (requires fun h0 ->
-    let gs0 = AL.v_arraylist pred1 pred2 pred3 (A.split_l md_region (u32_to_sz md_count_v)) (US.v idx1) (US.v idx2) (US.v idx3) h0 in
+    let gs0 = AL.v_arraylist pred1 pred2 pred3 pred4
+      (A.split_l md_region (u32_to_sz md_count_v))
+      (US.v idx1) (US.v idx2) (US.v idx3) (US.v idx4) h0 in
     let diff' = A.offset (A.ptr_of ptr) - A.offset (A.ptr_of slab_region) in
     0 <= diff' /\
     //diff' < (U32.v page_size) * (U32.v page_size) /\
@@ -931,10 +948,11 @@ let deallocate_slab'
     sel r1 h0 == idx1 /\
     sel r2 h0 == idx2 /\
     sel r3 h0 == idx3 /\
+    sel r4 h0 == idx4 /\
     U32.v md_count_v <> AL.null /\
     md_count_v == sel md_count h0 /\
     ALG.dataify gs0 `Seq.equal` G.reveal md_region_lv /\
-    ALG.partition #AL.status gs0 (US.v idx1) (US.v idx2) (US.v idx3)
+    ALG.partition #AL.status gs0 (US.v idx1) (US.v idx2) (US.v idx3) (US.v idx4)
   )
   (ensures fun _ _ _ -> True)
   =
@@ -952,41 +970,45 @@ let deallocate_slab'
     assert (A.offset (A.ptr_of ptr) - A.offset (A.ptr_of (slab_array (A.split_r slab_region 0sz) pos)) >= 0);
     assert (A.offset (A.ptr_of ptr) - A.offset (A.ptr_of (slab_array (A.split_r slab_region 0sz) pos)) < U32.v page_size);
     // selector equality propagation
-    let gs0 = gget (AL.varraylist pred1 pred2 pred3 (A.split_l md_region (u32_to_sz md_count_v)) (US.v idx1) (US.v idx2) (US.v idx3)) in
+    let gs0 = gget (AL.varraylist pred1 pred2 pred3 pred4
+      (A.split_l md_region (u32_to_sz md_count_v))
+      (US.v idx1) (US.v idx2) (US.v idx3) (US.v idx4)) in
     ALG.lemma_dataify_index #AL.status gs0 (U32.v pos);
     let status1 = AL.read_in_place
         (A.split_l md_region (u32_to_sz md_count_v))
-        (US.v idx1) (US.v idx2) (US.v idx3) (u32_to_sz pos) in
+        (US.v idx1) (US.v idx2) (US.v idx3) (US.v idx4) (u32_to_sz pos) in
     if (U32.eq status1 2ul) then (
       let b = deallocate_slab_aux_1 ptr size_class
         (A.split_r slab_region 0sz) md_bm_region md_region
-        md_count r1 r2 r3
-        md_count_v md_region_lv idx1 idx2 idx3 pos' in
+        md_count r1 r2 r3 r4
+        md_count_v md_region_lv idx1 idx2 idx3 idx4 pos' in
       pack_right_and_refactor_vrefine_dep
         size_class slab_region md_bm_region md_region md_count
-        r1 r2 r3 md_count_v;
+        r1 r2 r3 r4 md_count_v;
       return b
     ) else if (U32.eq status1 1ul) then (
       let b = deallocate_slab_aux_2 ptr size_class
         (A.split_r slab_region 0sz) md_bm_region md_region
-        md_count r1 r2 r3
-        md_count_v md_region_lv idx1 idx2 idx3 pos' in
+        md_count r1 r2 r3 r4
+        md_count_v md_region_lv idx1 idx2 idx3 idx4 pos' in
       pack_right_and_refactor_vrefine_dep
         size_class slab_region md_bm_region md_region md_count
-        r1 r2 r3 md_count_v;
+        r1 r2 r3 r4 md_count_v;
       return b
     ) else (
       deallocate_slab_fail ptr size_class
         slab_region md_bm_region md_region
-        md_count r1 r2 r3
-        md_count_v md_region_lv idx1 idx2 idx3
+        md_count r1 r2 r3 r4
+        md_count_v md_region_lv idx1 idx2 idx3 idx4
     )
   ) else (
     deallocate_slab_fail ptr size_class
       slab_region md_bm_region md_region
-      md_count r1 r2 r3
-      md_count_v md_region_lv idx1 idx2 idx3
+      md_count r1 r2 r3 r4
+      md_count_v md_region_lv idx1 idx2 idx3 idx4
   )
+
+// checkpoint
 
 #push-options "--compat_pre_typed_indexed_effects --z3rlimit 150"
 let deallocate_slab
@@ -996,21 +1018,21 @@ let deallocate_slab
   (md_bm_region: array U64.t{A.length md_bm_region = U32.v metadata_max * 4})
   (md_region: array AL.cell{A.length md_region = U32.v metadata_max})
   (md_count: ref U32.t)
-  (r1 r2 r3: ref US.t)
+  (r1 r2 r3 r4: ref US.t)
   : Steel bool
   (
     A.varray ptr `star`
     vrefinedep
       (vptr md_count)
       vrefinedep_prop
-      (size_class_vprop_aux size_class slab_region md_bm_region md_region r1 r2 r3)
+      (size_class_vprop_aux size_class slab_region md_bm_region md_region r1 r2 r3 r4)
   )
   (fun b ->
     (if b then emp else A.varray ptr) `star`
     vrefinedep
       (vptr md_count)
       vrefinedep_prop
-      (size_class_vprop_aux size_class slab_region md_bm_region md_region r1 r2 r3)
+      (size_class_vprop_aux size_class slab_region md_bm_region md_region r1 r2 r3 r4)
   )
   (requires fun _ ->
     let diff' = A.offset (A.ptr_of ptr) - A.offset (A.ptr_of slab_region) in
@@ -1026,14 +1048,14 @@ let deallocate_slab
     = elim_vrefinedep
       (vptr md_count)
       vrefinedep_prop
-      (size_class_vprop_aux size_class slab_region md_bm_region md_region r1 r2 r3) in
+      (size_class_vprop_aux size_class slab_region md_bm_region md_region r1 r2 r3 r4) in
 
   let md_count_v_ = read md_count in
 
   change_equal_slprop
-    (size_class_vprop_aux size_class slab_region md_bm_region md_region r1 r2 r3 (G.reveal md_count_v))
+    (size_class_vprop_aux size_class slab_region md_bm_region md_region r1 r2 r3 r4 (G.reveal md_count_v))
     (left_vprop size_class (A.split_r slab_region 0sz) md_bm_region md_region
-      r1 r2 r3 md_count_v_ `star`
+      r1 r2 r3 r4 md_count_v_ `star`
     right_vprop (A.split_r slab_region 0sz) md_bm_region md_region md_count_v_ `star`
     A.varrayp (A.split_l slab_region 0sz) halfp);
 
@@ -1041,49 +1063,54 @@ let deallocate_slab
   let x
     : G.erased _
     = elim_vdep
-    (left_vprop1 md_region r1 r2 r3 md_count_v_)
-    (left_vprop_aux size_class (A.split_r slab_region 0sz) md_bm_region md_region r1 r2 r3 md_count_v_) in
+    (left_vprop1 md_region r1 r2 r3 r4 md_count_v_)
+    (left_vprop_aux size_class (A.split_r slab_region 0sz) md_bm_region md_region r1 r2 r3 r4 md_count_v_) in
 
   change_equal_slprop
-    (left_vprop1 md_region r1 r2 r3 md_count_v_)
-    (ind_varraylist pred1 pred2 pred3
+    (left_vprop1 md_region r1 r2 r3 r4 md_count_v_)
+    (ind_varraylist pred1 pred2 pred3 pred4
       (A.split_l md_region (u32_to_sz md_count_v_))
-       r1 r2 r3);
+       r1 r2 r3 r4);
 
   let idxs
     : G.erased _
     = elim_vdep
-      (vptr r1 `star` vptr r2 `star` vptr r3)
-      (ind_varraylist_aux pred1 pred2 pred3 (A.split_l md_region (u32_to_sz md_count_v_)))
+      (vptr r1 `star` vptr r2 `star` vptr r3 `star` vptr r4)
+      (ind_varraylist_aux pred1 pred2 pred3 pred4 (A.split_l md_region (u32_to_sz md_count_v_)))
   in
   let idx1_ = read r1 in
   let idx2_ = read r2 in
   let idx3_ = read r3 in
+  let idx4_ = read r4 in
 
   elim_vrefine
-    (ind_varraylist_aux2 pred1 pred2 pred3 (A.split_l md_region (u32_to_sz md_count_v_)) idxs)
-    (ind_varraylist_aux_refinement pred1 pred2 pred3 (A.split_l md_region (u32_to_sz md_count_v_)) idxs);
+    (ind_varraylist_aux2 pred1 pred2 pred3 pred4
+      (A.split_l md_region (u32_to_sz md_count_v_)) idxs)
+    (ind_varraylist_aux_refinement pred1 pred2 pred3 pred4
+      (A.split_l md_region (u32_to_sz md_count_v_)) idxs);
 
   change_slprop_rel
-    (AL.varraylist pred1 pred2 pred3
+    (AL.varraylist pred1 pred2 pred3 pred4
       (A.split_l md_region (u32_to_sz md_count_v_))
-      (US.v (fst (fst (G.reveal idxs))))
+      (US.v (fst (fst (fst (G.reveal idxs)))))
+      (US.v (snd (fst (fst (G.reveal idxs)))))
       (US.v (snd (fst (G.reveal idxs))))
       (US.v (snd (G.reveal idxs))))
-    (AL.varraylist pred1 pred2 pred3
+    (AL.varraylist pred1 pred2 pred3 pred4
       (A.split_l md_region (u32_to_sz md_count_v_))
-      (US.v idx1_) (US.v idx2_) (US.v idx3_))
+      (US.v idx1_) (US.v idx2_) (US.v idx3_) (US.v idx4_))
     (fun x y -> x == y)
     (fun _ ->
-      assert (fst (fst (G.reveal idxs)) == idx1_);
-      assert (snd (fst (G.reveal idxs)) == idx2_);
-      assert (snd (G.reveal idxs) = idx3_)
+      assert (fst (fst (fst (G.reveal idxs))) == idx1_);
+      assert (snd (fst (fst (G.reveal idxs))) == idx2_);
+      assert (snd (fst (G.reveal idxs)) == idx3_);
+      assert (snd (G.reveal idxs) = idx4_)
     );
 
   let x' : G.erased (Seq.lseq AL.status (U32.v md_count_v_)) = ALG.dataify (dsnd x) in
 
   change_equal_slprop
-    (left_vprop_aux size_class (A.split_r slab_region 0sz) md_bm_region md_region r1 r2 r3 md_count_v_ x)
+    (left_vprop_aux size_class (A.split_r slab_region 0sz) md_bm_region md_region r1 r2 r3 r4 md_count_v_ x)
     (starseq
       #(pos:U32.t{U32.v pos < U32.v md_count_v_})
       #(t size_class)
@@ -1093,6 +1120,6 @@ let deallocate_slab
   let diff = A.ptrdiff ptr (A.split_l slab_region 0sz) in
 
   let b = deallocate_slab' ptr size_class
-    slab_region md_bm_region md_region md_count r1 r2 r3
-    md_count_v_ x' idx1_ idx2_ idx3_ diff in
+    slab_region md_bm_region md_region md_count r1 r2 r3 r4
+    md_count_v_ x' idx1_ idx2_ idx3_ idx4_ diff in
   return b
